ROOT
@@ -1,6 +1,8 @@
 session "Goblint_Formalization" in "src" = "HOL-IMP" +
   description "Isabelle/HOL formalization of the Goblint static analysis pipeline"
   options [quick_and_dirty]
+  sessions
+    Top_Down_Solver
   directories
     "IMP2"
     "CFG"
